Challenge/Modexp/Submission/Proofs/Bytecode/Artifact.lean
@@ -1270,7 +1270,7 @@ def submissionInstructions : List Instr :=
  YulEvmCompiler.Instr.push 2 1024,
  YulEvmCompiler.Instr.push 2 3072,
  YulEvmCompiler.Instr.push 2 1024,
- YulEvmCompiler.Instr.push 2 2467,
+ YulEvmCompiler.Instr.push 2 5029,
  YulEvmCompiler.Instr.op (EvmSemantics.Operation.StackMemFlow (EvmSemantics.Operation.StackMemFlowOps.JUMP)),
  YulEvmCompiler.Instr.op (EvmSemantics.Operation.StackMemFlow (EvmSemantics.Operation.StackMemFlowOps.JUMPDEST)),
  YulEvmCompiler.Instr.push 1 1,
